> Solve for $x$: $\frac{1}{2}x + \frac{1}{3}x - 2 [\frac{x-2}{4}] \geq 2 (x - 1) + 3x$.

--------------------------------

$\frac{1}{2}x + \frac{1}{3}x - 2 [\frac{x-2}{4}] \geq 2 (x - 1) + 3x$

$\Rightarrow (\frac{1}{2} + \frac{1}{3})x - 2 [\frac{x}{4} - \frac{1}{2}] \geq 2x - 2 + 3x$

$\Rightarrow \frac{5}{6}x - \frac{x}{2} + 1 \geq 5x - 2$

$\Rightarrow \frac{5}{6}x - \frac{x}{2} - 5x \geq - 1 - 2$

$\Rightarrow (\frac{5}{6} - \frac{1}{2} - 5)x \geq -3$

$\Rightarrow (\frac{5 - 3 - 30}{6})x \geq -3$

$\Rightarrow (\frac{-28}{6})x \geq -3$

$\Rightarrow \frac{-14}{3}x \geq -3$

$\Rightarrow x \leq \frac{-3}{14} \times (-3)$

$\Rightarrow x \leq \frac{9}{14}$